generic/Zeta.AppSimulate.Helper.fsti
@@ -1,0 +1,19 @@
+module Zeta.AppSimulate.Helper
+
+open Zeta.App
+open Zeta.AppSimulate
+(* Helper lemmas for reasoning about app simulate *)
+
+(* running a function with arity 0 leaves the state unchanged since the function does not
+ * read/write from/to the state *)
+val simulate_arity0_leaves_state_unchanged
+  (#aprm: app_params)
+  (fncall: appfn_call aprm)
+  (st: app_state aprm.adm)
+  (k: app_key aprm.adm)
+  : Lemma (requires (let fid = fncall.fid_c in
+                     appfn_arity fid = 0))
+          (ensures (let o = simulate_step fncall st in
+                    Some? o ==>
+                    (let st',_ = Some?.v o in
+                     st k = st' k)))
